feat(library/init/meta/smt_tactic): add assert/assertv/define/definev/pose/note for smt_tactic

src/library/tactic/assert_tactic.cpp
@@ -8,9 +8,10 @@ Author: Leonardo de Moura
 #include "library/vm/vm_name.h"
 #include "library/vm/vm_expr.h"
 #include "library/tactic/tactic_state.h"
+#include "library/tactic/intro_tactic.h"
 
 namespace lean {
-vm_obj assert_define(bool is_assert, name const & n, expr const & t, tactic_state const & s) {
+vm_obj assert_define_core(bool is_assert, name const & n, expr const & t, tactic_state const & s) {
     optional<metavar_decl> g = s.get_main_goal_decl();
     if (!g) return mk_no_goals_exception(s);
     type_context ctx     = mk_type_context_for(s);
@@ -24,31 +25,30 @@ vm_obj assert_define(bool is_assert, name const & n, expr const & t, tactic_stat
     local_context lctx   = g->get_context();
     metavar_context mctx = ctx.mctx();
     expr new_M_1         = mctx.mk_metavar_decl(lctx, t);
-    expr l;
-    if (is_assert)
-        l = lctx.mk_local_decl(n, t);
-    else
-        l = lctx.mk_local_decl(n, t, new_M_1);
-    expr new_M_2         = mctx.mk_metavar_decl(lctx, g->get_type());
-    expr new_val;
-    if (is_assert)
-        new_val = mk_app(mk_lambda(n, t, mk_delayed_abstraction(new_M_2, mlocal_name(l))), new_M_1);
-    else
-        new_val = mk_let(n, t, new_M_1, mk_delayed_abstraction(new_M_2, mlocal_name(l)));
+    expr new_M_2, new_val;
+    if (is_assert) {
+        expr new_target  = mk_pi(n, t, g->get_type());
+        new_M_2          = mctx.mk_metavar_decl(lctx, new_target);
+        new_val          = mk_app(new_M_2, new_M_1);
+    } else {
+        expr new_target  = mk_let(n, t, new_M_1, g->get_type());
+        new_M_2          = mctx.mk_metavar_decl(lctx, new_target);
+        new_val          = new_M_2;
+    }
     mctx.assign(head(s.goals()), new_val);
     list<expr> new_gs    = cons(new_M_1, cons(new_M_2, tail(s.goals())));
     return mk_tactic_success(set_mctx_goals(s, mctx, new_gs));
 }
 
-vm_obj tactic_assert(vm_obj const & n, vm_obj const & t, vm_obj const & s) {
-    return assert_define(true, to_name(n), to_expr(t), to_tactic_state(s));
+vm_obj tactic_assert_core(vm_obj const & n, vm_obj const & t, vm_obj const & s) {
+    return assert_define_core(true, to_name(n), to_expr(t), to_tactic_state(s));
 }
 
-vm_obj tactic_define(vm_obj const & n, vm_obj const & t, vm_obj const & s) {
-    return assert_define(false, to_name(n), to_expr(t), to_tactic_state(s));
+vm_obj tactic_define_core(vm_obj const & n, vm_obj const & t, vm_obj const & s) {
+    return assert_define_core(false, to_name(n), to_expr(t), to_tactic_state(s));
 }
 
-vm_obj assertv_definev(bool is_assert, name const & n, expr const & t, expr const & v, tactic_state const & s) {
+vm_obj assertv_definev_core(bool is_assert, name const & n, expr const & t, expr const & v, tactic_state const & s) {
     optional<metavar_decl> g = s.get_main_goal_decl();
     if (!g) return mk_no_goals_exception(s);
     type_context ctx     = mk_type_context_for(s);
@@ -67,35 +67,43 @@ vm_obj assertv_definev(bool is_assert, name const & n, expr const & t, expr cons
     }
     local_context lctx   = g->get_context();
     metavar_context mctx = ctx.mctx();
-    expr l;
-    if (is_assert)
-        l = lctx.mk_local_decl(n, t);
-    else
-        l = lctx.mk_local_decl(n, t, v);
-    expr new_M           = mctx.mk_metavar_decl(lctx, g->get_type());
-    expr new_val;
-    if (is_assert)
-        new_val = mk_app(mk_lambda(n, t, mk_delayed_abstraction(new_M, mlocal_name(l))), v);
-    else
-        new_val = mk_let(n, t, v, mk_delayed_abstraction(new_M, mlocal_name(l)));
+    expr new_M, new_val;
+    if (is_assert) {
+        expr new_target  = mk_pi(n, t, g->get_type());
+        new_M            = mctx.mk_metavar_decl(lctx, new_target);
+        new_val          = mk_app(new_M, v);
+    } else {
+        expr new_target  = mk_let(n, t, v, g->get_type());
+        new_M            = mctx.mk_metavar_decl(lctx, new_target);
+        new_val          = new_M;
+    }
     mctx.assign(head(s.goals()), new_val);
     list<expr> new_gs    = cons(new_M, tail(s.goals()));
     return mk_tactic_success(set_mctx_goals(s, mctx, new_gs));
 }
 
-vm_obj tactic_assertv(vm_obj const & n, vm_obj const & e, vm_obj const & pr, vm_obj const & s) {
-    return assertv_definev(true, to_name(n), to_expr(e), to_expr(pr), to_tactic_state(s));
+vm_obj tactic_assertv_core(vm_obj const & n, vm_obj const & e, vm_obj const & pr, vm_obj const & s) {
+    return assertv_definev_core(true, to_name(n), to_expr(e), to_expr(pr), to_tactic_state(s));
 }
 
-vm_obj tactic_definev(vm_obj const & n, vm_obj const & e, vm_obj const & pr, vm_obj const & s) {
-    return assertv_definev(false, to_name(n), to_expr(e), to_expr(pr), to_tactic_state(s));
+vm_obj tactic_definev_core(vm_obj const & n, vm_obj const & e, vm_obj const & pr, vm_obj const & s) {
+    return assertv_definev_core(false, to_name(n), to_expr(e), to_expr(pr), to_tactic_state(s));
+}
+
+vm_obj assertv_definev(bool is_assert, name const & n, expr const & t, expr const & v, tactic_state const & s) {
+    vm_obj r = assertv_definev_core(is_assert, n, t, v, s);
+    if (optional<tactic_state> const & s2 = is_tactic_success(r)) {
+        return intro(n, *s2);
+    } else {
+        return r;
+    }
 }
 
 void initialize_assert_tactic() {
-    DECLARE_VM_BUILTIN(name({"tactic", "assert"}),  tactic_assert);
-    DECLARE_VM_BUILTIN(name({"tactic", "assertv"}), tactic_assertv);
-    DECLARE_VM_BUILTIN(name({"tactic", "define"}),  tactic_define);
-    DECLARE_VM_BUILTIN(name({"tactic", "definev"}), tactic_definev);
+    DECLARE_VM_BUILTIN(name({"tactic", "assert_core"}),  tactic_assert_core);
+    DECLARE_VM_BUILTIN(name({"tactic", "assertv_core"}), tactic_assertv_core);
+    DECLARE_VM_BUILTIN(name({"tactic", "define_core"}),  tactic_define_core);
+    DECLARE_VM_BUILTIN(name({"tactic", "definev_core"}), tactic_definev_core);
 }
 
 void finalize_assert_tactic() {
