src/library/tactic/assert_tactic.h
@@ -7,7 +7,8 @@ Author: Leonardo de Moura
 #pragma once
 #include "library/tactic/tactic_state.h"
 namespace lean {
-vm_obj assert_define(bool is_assert, name const & n, expr const & t, tactic_state const & s);
+vm_obj assert_define_core(bool is_assert, name const & n, expr const & t, tactic_state const & s);
+vm_obj assertv_definev_core(bool is_assert, name const & n, expr const & t, expr const & v, tactic_state const & s);
 vm_obj assertv_definev(bool is_assert, name const & n, expr const & t, expr const & v, tactic_state const & s);
 void initialize_assert_tactic();
 void finalize_assert_tactic();
