tests/lean/run/smt_assert_define.lean
@@ -1,0 +1,22 @@
+open smt_tactic
+
+example (a b c : nat) : a = b + 0 → a + c = b + c :=
+by using_smt $ do
+  pr ← tactic.to_expr `(add_zero b),
+  note `h pr,
+  trace_state, return ()
+
+constant p : nat → nat → Prop
+constant f : nat → nat
+axiom pf (a : nat) : p (f a) (f a) → p a a
+
+example (a b c : nat) : a = b → p (f a) (f b) → p a b :=
+by using_smt $ do
+  t ← tactic.to_expr `(p (f a) (f a)),
+  assert `h t,  -- assert automatically closed the new goal
+  trace_state,
+  tactic.trace "-----",
+  pr ← tactic.to_expr `(pf _ h),
+  note `h2 pr,
+  trace_state,
+  return ()
